Alive/Template.lean
@@ -18,64 +18,140 @@ inductive val
 | int : (w : Width) → Int → val
 | pair : val → val → val
 | triple : val → val → val → val
+| error : val
 
-instance : Inhabited val where
-  default := .int 0 0
+class Pointed (α : Type) where
+  point : α
 
--- @Chris: these are DUMMY DEFINITIONS! They need to be modified.
+def Pointed.morphism [Pointed α] [Pointed β] (f: α → β) : Prop :=
+  f point = point
+
+def val.binaryIntFunction (w : Width) (f : Int → Int → Int)
+ (x : val) (y : val) : val :=
+  match x with
+  | .int w1 v1 =>
+     match y with
+     | .int w2 v2 =>
+         if W1 : w1 = w then
+           if W2 : w2 = w then
+             .int w <| f v1 v2
+           else error
+         else error
+     | _ => .error
+  | _ => .error
+
+@[simp, aesop norm simp]
+theorem val.binaryIntFuction_l_w_neq (H : w1 ≠ w) :
+  val.binaryIntFunction w f (.int w1 v1) y = .error := by {
+    simp[binaryIntFunction, H]; cases y <;> simp;
+
+}
+
+@[simp, aesop norm simp]
+theorem val.binaryIntFuction_r_w_neq (H : w2 ≠ w) :
+  val.binaryIntFunction w f x (.int w2 v2)  = .error := by {
+    simp[binaryIntFunction, H]; cases x <;> simp;
+}
+
+@[simp]
+theorem val.binaryIntFunction_l_pair :
+   val.binaryIntFunction w f (.pair x1 x2) y = .error := by {
+  simp[binaryIntFunction];
+}
+
+@[simp]
+theorem val.binaryIntFunction_l_triple :
+   val.binaryIntFunction w f (.triple x1 x2 x3) y = .error := by {
+  simp[binaryIntFunction];
+}
+
+@[simp]
+theorem val.binaryIntFunction_l_error :
+   val.binaryIntFunction w f .error y = .error := by {
+  simp[binaryIntFunction];
+}
+
+@[simp]
+theorem val.binaryIntFunction_r_pair :
+   val.binaryIntFunction w f x (.pair y1 y2) = .error := by {
+  simp[binaryIntFunction];
+  cases x <;> simp;
+}
+
+@[simp]
+theorem val.binaryIntFunction_r_triple :
+   val.binaryIntFunction w f x (.triple y1 y2 y3) = .error := by {
+  simp[binaryIntFunction];
+  cases x <;> simp;
+}
+
+@[simp]
+theorem val.binaryIntFunction_r_error :
+   val.binaryIntFunction w f x .error = .error := by {
+  simp[binaryIntFunction]; cases x <;> simp
+}
+
+
+def pow2 : Nat → Nat
+| 0 => 1
+| n+1 => 2 * pow2 n
+
+@[simp]
 def val.add (w : Width) (x y : val) : val :=
-  match x with
-  | .int _w1 v1 =>
-    match y with
-    | .int _w2 v2 => .int 0 <| (v1 + v2) % w
-    | _ => default
-  | _ => default
+  val.binaryIntFunction w (fun x y => (x + y) % pow2 w) x y
+
+@[simp]
 def val.and (w : Width) (x y : val) : val :=
-  match x with
-  | .int _w1 v1 =>
-    match y with
-    | .int _w2 v2 => .int 0 <| (Int.land v1 v2) % w
-    | _ => default
-  | _ => default
+  val.binaryIntFunction w (fun x y => (Int.land x y) % pow2 w) x y
+
 def val.negate (w : Width) (x : val) : val :=
   match x with
   | .int _w1 v1 => .int 0 <| (- v1) % w
-  | _ => default
+  | _ => .error
+
+@[simp]
+theorem val.negate.pair : val.negate w (.pair x1 x2) = .error := by {
+  simp[negate];
+}
+
+@[simp]
+theorem val.negate.triple : val.negate w (.triple x1 x2 x3) = .error := by {
+  simp[negate];
+}
+
+
+@[simp]
+theorem val.negate.error : val.negate w (.error) = .error := by {
+  simp[negate];
+}
+
+@[simp]
 def val.or (w : Width) (x y : val) : val :=
-  match x with
-  | .int _w1 v1 =>
-    match y with
-    | .int _w2 v2 => .int 0 <| (Int.lor v1 v2) % w
-    | _ => default
-  | _ => default
+  val.binaryIntFunction w (fun x y => (Int.lor x y) % pow2 w) x y
+
+
+@[simp]
 def val.sub (w : Width) (x y : val) : val :=
-  match x with
-  | .int _w1 v1 =>
-    match y with
-    | .int _w2 v2 => .int 0 <| (Int.sub v1 v2) % w
-    | _ => default
-  | _ => default
+  val.binaryIntFunction w (fun x y => (x - y) % pow2 w) x y
+
+@[simp]
 def val.xor (w : Width) (x y : val) : val :=
-  match x with
-  | .int _w1 v1 =>
-    match y with
-    | .int _w2 v2 => .int 0 <| (Int.lxor' v1 v2) % w
-    | _ => default
-  | _ => default
+  val.binaryIntFunction w (fun x y => (Int.lxor' x y) % pow2 w) x y
 
 @[simp]
 def op.eval (o : op) (v : val) (_rgn : val → val) : val :=
  match o with
  | .const w i => val.int w i
- | .add w => match v with | .pair x y => val.add w x y | _ => default
- | .and w => match v with | .pair x y => val.and w x y | _ => default
+ | .add w => match v with | .pair x y => val.add w x y | _ => .error
+ | .and w => match v with | .pair x y => val.and w x y | _ => .error
  | .negate w => val.negate w v
- | .or w => match v with | .pair x y => val.or w x y | _ => default
- | .sub w => match v with | .pair x y => val.sub w x y | _ => default
- | .xor w => match v with | .pair x y => val.xor w x y | _ => default
+ | .or w => match v with | .pair x y => val.or w x y | _ => .error
+ | .sub w => match v with | .pair x y => val.sub w x y | _ => .error
+ | .xor w => match v with | .pair x y => val.xor w x y | _ => .error
 
 @[simp]
 instance S : UserSemantics op val where
+  default := .error
   eval := op.eval
   valPair := val.pair
   valTriple := val.triple
